src/cbor/pulse/CBOR.Pulse.API.Det.C.fsti
@@ -116,7 +116,7 @@ val cbor_det_mk_simple_value () : mk_simple_t cbor_det_match
 val cbor_det_mk_int64 () : mk_int64_t cbor_det_match
 val cbor_det_mk_tagged () : mk_tagged_t cbor_det_match
 
-val cbor_det_mk_string_from_array (_: unit) : mk_string_from_array_t cbor_det_match
+val cbor_det_mk_string_from_arrayptr (_: unit) : mk_string_from_arrayptr_t cbor_det_match
 
 val cbor_det_mk_array_from_array (_: unit) : mk_array_from_array_t cbor_det_match
 
